SATnat.v
@@ -1,23 +1,14 @@
 Set Implicit Arguments.
-
+Require Import basic Can Sat.
 Require Import ZF ZFind_nat.
 Import IZF.
+Module Lc:=Lambda.
 
 (* Saturated sets constructions related to natural numbers *)
 
-Record num := mkNat { number :> set; is_num : number \in NAT }.
-
-Definition eqnum (x y:num) := x == y.
-
-Definition ZEROt := mkNat ZERO_typ.
-Definition SUCCt n := mkNat (SUCC_typ _ (is_num n)).
-
-Require Import basic Can Sat.
-Module Lc:=Lambda.
-
 Record family := mkFam {
-  fam :> num -> SAT;
-  fam_mrph : forall x y, eqnum x y -> eqSAT (fam x) (fam y)
+  fam :> set -> SAT;
+  fam_mrph : forall x y,  x \in NAT -> x == y -> eqSAT (fam x) (fam y)
 }.
 
 Definition dflt_family : family.
@@ -26,62 +17,30 @@ reflexivity.
 Defined.
 
 Definition eqfam (A B:family) :=
-  forall x y, eqnum x y -> eqSAT (A x) (B y).
+  forall x y, x \in NAT -> x == y -> eqSAT (A x) (B y).
 
-Definition fNAT (A:family) (k:num) :=
+Definition fNAT (A:family) (k:set) :=
   interSAT
     (fun P:family =>
-      prodSAT (P ZEROt)
-     (prodSAT (interSAT (fun n => prodSAT (A n) (prodSAT (P n) (P (SUCCt n)))))
+      prodSAT (P ZERO)
+     (prodSAT (interSAT (fun n:{n|n\in NAT} => let n:=proj1_sig n in
+               prodSAT (A n) (prodSAT (P n) (P (SUCC n)))))
               (P k))).
 
 Lemma fNAT_morph : forall A B, eqfam A B ->
-  forall x y, eqnum x y -> eqSAT (fNAT A x) (fNAT B y).
+  forall x y, x \in NAT -> x == y -> eqSAT (fNAT A x) (fNAT B y).
 intros.
 unfold fNAT.
 apply interSAT_morph.
-split; intros.
- exists x0.
+apply indexed_relation_id; intros.
+apply prodSAT_morph.
+ reflexivity.
+
  apply prodSAT_morph.
-  reflexivity.
+  apply interSAT_morph_subset; simpl proj1_sig; intros; auto with *.
+  apply prodSAT_morph; auto with *.
 
-  apply prodSAT_morph.
-   apply interSAT_morph.
-   split; intros.
-    exists x1.
-    apply prodSAT_morph.
-     apply H; red; reflexivity.
-
-     reflexivity.
-
-    exists y0.
-    apply prodSAT_morph.
-     apply H; red; reflexivity.
-
-     reflexivity.
-
-   apply (fam_mrph x0); trivial.
-
- exists y0.
- apply prodSAT_morph.
-  reflexivity.
-
-  apply prodSAT_morph.
-   apply interSAT_morph.
-   split; intros.
-    exists x0.
-    apply prodSAT_morph.
-     apply H; red; reflexivity.
-
-     reflexivity.
-
-    exists y1.
-    apply prodSAT_morph.
-     apply H; red; reflexivity.
-
-     reflexivity.
-
-   apply (fam_mrph y0); trivial.
+  apply fam_mrph; trivial.
 Qed.
 
 Definition fNATf (A:family) : family.
@@ -95,30 +54,29 @@ Defined.
 Lemma fNAT_def : forall t A k,
   inSAT t (fNAT A k) <->
   forall (P:family) f g,
-  inSAT f (P ZEROt) ->
-  (forall n m y, inSAT m (A n) -> inSAT y (P n) -> inSAT (Lc.App2 g m y) (P (SUCCt n))) ->
+  inSAT f (P ZERO) ->
+  (forall n m y, n \in NAT -> inSAT m (A n) -> inSAT y (P n) -> inSAT (Lc.App2 g m y) (P (SUCC n))) ->
   inSAT (Lc.App2 t f g) (P k).
 unfold fNAT.
 split; intros.
  apply interSAT_elim with (x:=P) in H.
- apply prodSAT_elim with (interSAT (fun n => prodSAT (A n) (prodSAT (P n) (P (SUCCt n))))).
-  apply prodSAT_elim with (2:=H0); trivial.
-
-  apply interSAT_intro; trivial; intros.
-  simpl.
-  do 2 red; intros.
-  apply H1; trivial.
+ apply prodSAT_elim with (interSAT (fun n:{n|n\in NAT} =>
+    let n:=proj1_sig n in prodSAT (A n) (prodSAT (P n) (P (SUCC n))))).
+ apply prodSAT_elim with (2:=H0); trivial.
+ apply interSAT_intro; trivial; intros.
+  exists ZERO; apply ZERO_typ.
+ destruct x as (n,?); simpl.
+ do 2 red; intros.
+ apply H1; trivial.
 
  apply interSAT_intro; intros.
   exists (fun _ => snSAT); reflexivity.
- simpl.
- do 2 red; intros.
- apply H with (P:=x); intros; trivial.
+ simpl; do 2 red; intros.
  destruct H1.
- do 2 red in H4.
- apply H4; auto.
+ apply H; trivial.
+ intros.
+ apply H2 with (x0:=exist (fun x => x\in NAT) n H3); trivial.
 Qed.
-
 
 Lemma fNAT_mono : forall (A B:family),
   (forall k, inclSAT (A k) (B k)) -> forall k, inclSAT (fNAT A k) (fNAT B k).
@@ -127,7 +85,7 @@ rewrite fNAT_def in H0 |- *; intros.
 apply H0; intros; auto.
 Qed.
 
-(* Fixpoint of fNAT *)
+(* Realizability relation of NAT: fixpoint of fNAT *)
 
 Definition cNAT : family.
 exists (fun n =>
@@ -170,34 +128,12 @@ split.
  apply cNAT_post.
 Qed.
 
-(* Realizability relation of natural numbers *)
-
-Definition realNat (n:set) (t:Lc.term) :=
-  exists H:n \in NAT, inSAT t (cNAT (mkNat H)).
-
-Lemma realNat_cand : forall n,
-  n \in NAT -> is_cand (fun t => realNat n t).
-intros.
-cut (is_cand (fun t => inSAT t (cNAT (mkNat H)))).
- apply is_cand_morph; red; intros.
- assert (forall (p : n \in NAT), eqSAT (cNAT (mkNat p)) (cNAT (mkNat H))).
-  intros.
-  apply fam_mrph; red; reflexivity.
- split; intros.
-  destruct H1.
-  rewrite H0 in H1; trivial.
-
-  exists H; trivial.
-
- exact (proj2_sig (cNAT (mkNat H))).
-Qed.
-
 (* Constructors *)
 
 (* interp of 0 *)
 Definition ZE := Lc.Abs (Lc.Abs (Lc.Ref 1)).
 
-Lemma fNAT_ZE : forall A, inSAT ZE (fNAT A ZEROt).
+Lemma fNAT_ZE : forall A, inSAT ZE (fNAT A ZERO).
 unfold fNAT, ZE; intros A.
 apply interSAT_intro; trivial.
 intro P.
@@ -207,15 +143,21 @@ apply prodSAT_intro; intros.
 unfold Lc.subst; rewrite Lc.simpl_subst; trivial; rewrite Lc.lift0; trivial.
 Qed.
 
+Lemma cNAT_ZE : inSAT ZE (cNAT ZERO).
+rewrite cNAT_eq.
+apply fNAT_ZE.
+Qed.
+
 (* interp of successor *)
 Definition SU := Lc.Abs (Lc.Abs (Lc.Abs
     (Lc.App2 (Lc.Ref 0) (Lc.Ref 2) (Lc.App2 (Lc.Ref 2) (Lc.Ref 1) (Lc.Ref 0))))).
 
 Lemma fNAT_SU : forall (A:family) n t,
+  n \in NAT ->
   inSAT t (A n) ->
   inSAT t (fNAT A n) ->
-  inSAT (Lc.App SU t) (fNAT A (SUCCt n)).
-intros.
+  inSAT (Lc.App SU t) (fNAT A (SUCC n)).
+intros A n t tyn H H0.
 unfold fNAT, SU.
 apply interSAT_intro; trivial.
 intros P.
@@ -227,7 +169,7 @@ apply prodSAT_intro; intros.
 unfold Lc.subst; simpl Lc.subst_rec; rewrite Lc.simpl_subst; trivial.
 apply prodSAT_intro; intros.
 unfold Lc.subst; simpl Lc.subst_rec; repeat rewrite Lc.simpl_subst; trivial; repeat rewrite Lc.lift0.
-specialize interSAT_elim with (x:=n) (1:=H3); intro.
+specialize interSAT_elim with (x:=exist (fun n=>n\in NAT) n tyn) (1:=H3); simpl proj1_sig; intro.
 specialize interSAT_elim with (x:=true) (1:=H1); intro.
 specialize interSAT_elim with (x:=false) (1:=H1); intro.
 specialize interSAT_elim with (x:=P) (1:=H6); intro.
@@ -239,12 +181,7 @@ apply prodSAT_elim with (A:=P n).
  apply prodSAT_elim with (1:=H7); trivial.
 Qed.
 
-Lemma cNAT_ZE : inSAT ZE (cNAT ZEROt).
-rewrite cNAT_eq.
-apply fNAT_ZE.
-Qed.
-
-Lemma cNAT_SU : forall n t, inSAT t (cNAT n) -> inSAT (Lc.App SU t) (cNAT (SUCCt n)). 
+Lemma cNAT_SU : forall n t, n \in NAT -> inSAT t (cNAT n) -> inSAT (Lc.App SU t) (cNAT (SUCC n)). 
 intros.
 rewrite cNAT_eq.
 apply fNAT_SU; trivial.
