SN_CC_Real.v
@@ -1,0 +1,787 @@
+Require Export Relations Wellfounded Compare_dec.
+Require Import Sat.
+Require Import ZF ZFcoc.
+Require Import ZFlambda.
+Import IZF.
+
+Set Implicit Arguments.
+
+(***********************************************************************************************)
+(* Proving the SN model requirements *)
+
+Module CCSN.
+
+(* Types are coded by a carrier set X and a realizability relation R
+   assigning a reducibility candidate to each element of the
+   domain.
+   This means that even non-computable functions have "realizers",
+   but no closed ones (it is the set of neutral terms).
+ *)
+Definition mkTY X R := couple X (cc_lam X (fun x => iSAT (R x))).
+
+Lemma mkTY_ext : forall X Y R R',
+  X == Y ->
+  (forall x x', x \in X -> x == x' -> eqSAT (R x) (R' x')) ->
+  mkTY X R == mkTY Y R'.
+unfold mkTY; intros.
+apply couple_morph; trivial.
+apply cc_lam_ext; auto.
+red; intros.
+apply iSAT_morph.
+auto.
+Qed.
+
+(* Accessing the set of values of a type: *)
+Definition El T := fst T.
+
+(* Accessing the realizability relation *)
+Definition Red T x := sSAT (cc_app (snd T) x) .
+
+Instance El_morph : morph1 El.
+Proof fst_morph.
+
+Instance Red_morph : Proper (eq_set==>eq_set==>eqSAT) Red.
+do 3 red; intros.
+unfold Red.
+apply sSAT_morph.
+rewrite H; rewrite H0; reflexivity.
+Qed.
+
+Lemma El_def : forall X R, El (mkTY X R) == X.
+unfold El,mkTY; intros.
+apply fst_def.
+Qed.
+
+Lemma Red_def : forall x X R,
+  (forall x x', x \in X -> x == x' -> eqSAT (R x) (R x')) ->
+  x \in X ->
+  eqSAT (Red (mkTY X R) x) (R x).
+intros.
+unfold Red, mkTY.
+rewrite snd_def.
+rewrite cc_beta_eq; auto.
+ apply iSAT_id.
+
+ do 2 red; intros.
+ apply iSAT_morph; auto.
+Qed.
+
+(* The realizability relation of a dependent product of domain type A
+   and co-domain family of types F for a  function f:
+   it is the intersection of all reducibility candidates {x}_A -> {f(x)}_F(x)
+   when x ranges A. *)
+Definition piSAT A (F:set->set) f :=
+  interSAT (fun p:{x|x \in El A} =>
+    prodSAT (Red A (proj1_sig p)) (Red (F (proj1_sig p)) (f (proj1_sig p)))).
+
+Lemma piSAT_morph : forall A B F F' f f',
+  A == B ->
+  eq_fun (El A) F F' ->
+  eq_fun (El A) f f' -> 
+  eqSAT (piSAT A F f) (piSAT B F' f').
+unfold piSAT; intros.
+apply interSAT_morph_subset; simpl; intros; auto with *.
+ rewrite H; reflexivity.
+
+ apply prodSAT_morph; auto with *.
+  apply Red_morph; auto with *.
+
+  apply Red_morph; auto with *.
+Qed.
+
+Definition prod A F :=
+  mkTY (cc_prod (El A) (fun x => El (F x))) (fun f => piSAT A F (cc_app f)).
+
+Lemma Red_prod : forall dom f F,
+    eq_fun (El dom) F F ->
+    f \in El (prod dom F) ->
+    eqSAT (Red (prod dom F) f) (piSAT dom F (cc_app f)).
+unfold prod; intros.
+rewrite El_def in H0; rewrite Red_def; trivial.
+ reflexivity.
+
+ do 2 red; intros.
+ apply piSAT_morph; auto with *.
+ red; intros; apply cc_app_morph; trivial.
+Qed.
+
+Definition lam A F := cc_lam (El A) F.
+
+Definition app := cc_app.
+
+Lemma prod_intro : forall dom f F,
+  ext_fun (El dom) f ->
+  ext_fun (El dom) F ->
+  (forall x, x \in El dom -> f x \in El (F x)) ->
+  lam dom f \in El (prod dom F).
+intros.
+unfold lam, prod, mkTY, El.
+rewrite fst_def.
+apply cc_prod_intro; intros; auto.
+do 2 red; intros.
+apply fst_morph; auto.
+Qed.
+
+
+Lemma prod_elim : forall dom f x F,
+  eq_fun (El dom) F F ->
+  f \in El (prod dom F) ->
+  x \in El dom ->
+  cc_app f x \in El (F x).
+intros dom f x F _ H.
+unfold prod, mkTY, El in H.
+rewrite fst_def in H.
+apply cc_prod_elim with (dom:=El dom) (F:=fun x => El(F x)); trivial.
+Qed.
+
+(* The type of propositions:
+   - propositions are types and do not interact with their surrounding context, so
+     the set of realizers of any proposition is SN
+   - all propositions are non-empty (and equal to True), but their set of
+     realizers must depend on the syntax of the propositions, because proofs compute.
+     The realizer sets can be any reducibility candidate.
+   Remark: we cannot have that all propositions are equal (they can differ on the
+   set of realizers). Otherwise True=(True->True) wold allow non normalizing terms
+   (e.g. Y).
+ *)
+Definition props :=
+  mkTY
+    (* The domain of props *)
+    (replSAT (fun A:SAT => mkTY (singl prf_trm) (fun _ => A)))
+    (* realizers of prop *)
+    (fun _ => snSAT).
+
+Lemma prop_repl_morph :
+  Proper (eqSAT ==> eq_set) (fun A => mkTY (singl prf_trm) (fun _ => A)).
+do 2 red; intros.
+apply couple_morph; try reflexivity.
+apply cc_lam_ext; auto with *.
+red; intros.
+apply iSAT_morph; trivial.
+Qed.
+Hint Resolve prop_repl_morph.
+
+
+(*
+Definition mkProp S :=
+  mkTy (power empty) (fun x t => inSAT t S).
+
+Lemma prop3 : forall S, Proper (eq_set ==> eq ==> iff) (fun _ t => inSAT t S).
+do 3 red; intros.
+subst y0; reflexivity.
+Qed.
+
+Lemma mkProp_def : forall x t S,
+  (x,t) \real mkProp S <-> x == empty /\ inSAT t S.
+intros.
+unfold mkProp.
+rewrite mkTy_def0.
+2:apply prop3.
+ setoid_replace (x \in power empty) with (x == empty);
+   auto with *.
+ rewrite power_ax.
+ split; intros.
+  apply empty_ext; red; intros.
+  generalize (H _ H0); apply empty_ax.
+
+  rewrite <- H; trivial.
+
+ intros _ _.
+ generalize (proj2_sig S); apply iff_impl.
+ apply is_cand_morph; red; intros.
+ reflexivity.
+Qed.
+
+Lemma El_mkProp : forall S, El (mkProp S) == power empty.
+intros.
+apply power_ext; intros.
+ rewrite El_def.
+ exists (Lc.Ref 0).
+ rewrite mkProp_def; split.
+  apply empty_ext; red; intros.
+  apply H in H0; elim empty_ax with x0; trivial.
+
+  apply varSAT.
+
+ rewrite El_def in H.
+ destruct H.
+ rewrite mkProp_def in H; destruct H.
+ rewrite H in H0; trivial.
+Qed.
+
+Lemma prop2 :
+  Proper (eq_set ==> eq ==> iff)
+    (fun P t => Lc.sn t /\ (exists S : SAT, P == mkProp S)).
+do 3 red; intros.
+subst y0.
+apply and_iff_morphism; auto with *.
+apply ex_morph; red; intros.
+rewrite H; reflexivity.
+Qed.
+
+Lemma props_def : forall x t,
+  (x,t) \real props <-> (exists S, x == mkProp S) /\ Lc.sn t.
+*)
+
+  Lemma Red_sort : forall x, x \in El props -> eqSAT (Red props x) snSAT.
+intros.
+unfold props.
+rewrite Red_def; auto with *.
+unfold props in H; rewrite El_def in H; trivial.
+Qed.
+
+(* Re-doing the impredicativity property in the case where we have no
+   empty propositions *)
+Lemma cc_impredicative_prod_non_empty : forall dom F,
+  ext_fun dom F ->
+  (forall x, x \in dom -> F x == singl prf_trm) ->
+  cc_prod dom F == singl prf_trm.
+Proof.
+intros.
+apply singl_ext; intros.
+ rewrite <- (cc_impredicative_lam dom (fun x => prf_trm)); intros.
+ 2:do 2 red; reflexivity.
+  apply cc_prod_intro; intros; auto.
+  apply H0 in H1; rewrite H1.
+  apply singl_intro.
+
+  reflexivity.
+
+ unfold cc_prod in H1.
+ rewrite replf_ax in H1; intros.
+  destruct H1 as (f,f_fun,z_lam).
+  rewrite z_lam; clear z z_lam.
+  apply cc_impredicative_lam; intros.
+   do 2 red; intros.
+   rewrite H2; reflexivity.
+
+   apply singl_elim.
+   fold prf_trm.
+   rewrite <- (H0 _ H1).
+   apply dep_func_elim with (1:=f_fun); trivial.
+
+  do 2 red; intros.
+  apply cc_lam_ext; try reflexivity.
+  red; intros.
+  apply app_morph; trivial.
+Qed.
+
+Lemma impredicative_prod : forall dom F,
+  ext_fun (El dom) F ->
+  (forall x, x \in El dom -> F x \in El props) ->
+  prod dom F \in El props.
+unfold props, mkTY, El; intros.
+rewrite fst_def.
+rewrite replSAT_ax; trivial.
+unfold prod, mkTY.
+exists (piSAT dom F (fun _ => prf_trm)).
+assert (forall x, x \in El dom -> El (F x) == singl prf_trm).
+ intros.
+ specialize H0 with (1:=H1).
+ rewrite fst_def in H0.
+ rewrite replSAT_ax in H0; trivial.
+ destruct H0 as (A,H0); rewrite H0.
+ unfold El; rewrite fst_def.
+ reflexivity.
+apply mkTY_ext.
+ apply cc_impredicative_prod_non_empty; intros; auto.
+ do 2 red; intros.
+ unfold El; apply fst_morph; auto.
+
+ intros.
+ apply piSAT_morph; auto with *.
+ red; intros.
+ apply singl_elim.
+ rewrite <- (H1 x0); trivial.
+ apply cc_prod_elim with (1:=H2); trivial.
+Qed.
+
+(* All propositions are inhabited: *)
+  Definition daimon := prf_trm.
+  Lemma daimon_false : prf_trm \in El (prod props (fun P => P)).
+setoid_replace prf_trm with (cc_lam (El props) (fun _ => prf_trm)).
+ unfold prod, mkTY, El; rewrite fst_def.
+ apply cc_prod_intro; intros.
+  do 2 red; reflexivity.
+
+  do 2 red; intros; apply fst_morph; trivial.
+  unfold props, mkTY in H.
+  rewrite fst_def in H.
+  rewrite replSAT_ax in H; trivial.
+  destruct H as (A, eq_x).
+  rewrite eq_x.
+  rewrite fst_def.
+  apply singl_intro.
+
+ symmetry.
+ apply cc_impredicative_lam; intros.
+  do 2 red; intros; reflexivity.
+  reflexivity.
+Qed.
+
+(* Module bureaucracy *)
+Definition X:=set.
+Definition eqX := eq_set.
+Definition eqX_equiv := eq_set_equiv.
+Definition inX x y := x \in El y.
+Lemma in_ext : Proper (eq_set==>eq_set==>iff) inX.
+apply morph_impl_iff2; auto with *.
+unfold inX; do 4 red; intros.
+rewrite <- H; rewrite <- H0; trivial.
+Qed.
+
+Definition eq_fun (x:X) (f1 f2:X->X) :=
+  forall y1 y2, y1 \in El x -> y1 == y2 -> f1 y1 == f2 y2.
+
+Lemma lam_ext :
+  forall x1 x2 f1 f2,
+  x1 == x2 ->
+  eq_fun x1 f1 f2 ->
+  lam x1 f1 == lam x2 f2.
+unfold lam; intros.
+apply cc_lam_ext; trivial.
+apply El_morph; trivial.
+Qed.
+
+Lemma app_ext: Proper (eqX ==> eqX ==> eqX) app.
+Proof cc_app_morph.
+
+Lemma prod_ext :
+  forall x1 x2 f1 f2,
+  x1 == x2 ->
+  eq_fun x1 f1 f2 ->
+  prod x1 f1 == prod x2 f2.
+unfold prod; intros.
+apply mkTY_ext; intros.
+ apply cc_prod_ext; auto.
+  apply El_morph; trivial.
+
+  red; intros.
+  apply El_morph; auto.
+
+ apply piSAT_morph; intros; auto.
+ red; intros.
+ apply cc_app_morph; trivial.
+Qed.
+
+Lemma beta_eq:
+  forall dom F x,
+  eq_fun dom F F ->
+  x \in El dom ->
+  app (lam dom F) x == F x.
+intros.
+unfold app, lam.
+rewrite cc_beta_eq; auto with *.
+Qed.
+
+End CCSN.
+Import CCSN.
+
+(* Checking module instantiation. *)
+(*
+Module __ <: CC_Model.
+  Include CCSN.
+End __.
+Module ___ <: RealSN_addon CCSN.
+  Include CCSN.
+End ___.
+*)
+
+
+(***********************************************************************************************)
+
+(* Building the generic model *)
+Require GenRealSN.
+Module SN := GenRealSN.MakeModel CCSN CCSN.
+Import SN.
+
+Module Lc := Lambda.
+
+(***********************************************************************************************)
+
+(* Consistency out of the strong normalization model *)
+
+(* Property of substitutivity: whenever a term-denotation contains
+   a free var, then it comes from the term-valuation *)
+Lemma tm_closed : forall k j M,
+  Lc.occur k (tm j M) -> ~ forall n, ~ Lc.occur k (j n).
+red; intros.
+rewrite Lc.occur_subst in H.
+rewrite <- tm_substitutive in H.
+rewrite <- tm_liftable in H.
+apply H; clear H.
+apply tm_morph; auto with *.
+red; red; intros.
+generalize (H0 a).
+rewrite Lc.occur_subst; intro.
+destruct (Lc.eqterm (Lc.lift_rec 1 (Lc.subst_rec (Lc.Abs (Lc.Ref 0)) (j a) k) k) (j a)); auto.
+elim H; trivial.
+Qed.
+
+(* If t belongs to all reducibility candidates, then it has a free variable *)
+Lemma neutral_not_closed :
+  forall t, (forall S, inSAT t S) -> exists k, Lc.occur k t.
+intros.
+assert (neu := H (exist _ _ Can.neutral_is_cand : SAT)).
+simpl in neu.
+destruct neu.
+destruct H1.
+destruct H2.
+destruct Lc.nf_neutral_open with (1:=H2) (2:=H3).
+exists x0.
+apply Lc.red_closed with x; auto.
+Qed.
+
+(* Another consistency proof.
+
+   What is original is that it is based on the strong normalization model which
+   precisely inhabits all types and propositions. We get out of this by noticing that
+   non provable propositions contain no closed realizers. So, by a substitutivity
+   invariant (realizers of terms typed in the empty context cannot introduce free
+   variables), we derive the impossibility to derive absurdity in the empty context.
+
+   The result is at the level of the model. See below for the proof that the actual syntax
+   (libraries Term and TypeJudge) can be mapped to the model.
+ *)
+Theorem consistency : forall M, ~ typ List.nil M (Prod prop (Ref 0)).
+red; intros.
+red in H.
+(* The valuation below contains only closed terms, and it interprets the
+   empty context *) 
+assert (val_ok List.nil (V.nil props) (I.nil (Lc.Abs (Lc.Ref 0)))).
+ red; intros.
+ destruct n; discriminate H0.
+apply H in H0.
+clear H.
+red in H0; simpl in_int in H0.
+destruct H0 as (_,H0).
+simpl int in H0.
+destruct H0.
+set (prf := tm (I.nil (Lc.Abs (Lc.Ref 0))) M) in H0.
+assert (forall S, inSAT (Lc.App prf (Lc.Abs (Lc.Ref 0))) S).
+ intros.
+ pose (P := mkTY (singl prf_trm) (fun _ => S)).
+ assert ([P, Lc.Abs (Lc.Ref 0)] \real props). 
+  assert (P \in El props).
+   unfold props; rewrite El_def.
+   rewrite replSAT_ax; auto.
+   exists S; reflexivity.
+  split; trivial.
+  rewrite Red_sort; auto.
+  apply Lc.sn_abs; auto.
+ assert (H2 := @prod_elim props (int(V.nil props) M) P (fun P=>P) prf (Lc.Abs (Lc.Ref 0))).
+ destruct H2; trivial.
+  red; auto.
+
+  split; trivial.
+ setoid_replace  S with (Red P (cc_app (int (V.nil props) M) P)); trivial.
+ unfold P; rewrite Red_def; auto with *.
+ apply eq_elim with (El P).
+  unfold P; rewrite El_def.
+  reflexivity.
+
+  unfold inX, prod in H.
+  rewrite El_def in H.
+  apply cc_prod_elim with (1:=H).
+  unfold props; rewrite El_def.
+  rewrite replSAT_ax; auto.
+  exists S; reflexivity.
+destruct (neutral_not_closed _ H1).
+inversion_clear H2.
+ apply tm_closed in H3.
+ apply H3.
+ red; intros.
+ unfold I.nil in H2; simpl in H2.
+ inversion_clear H2.
+ inversion H4.
+
+ inversion_clear H3.
+ inversion H2.
+Qed.
+
+Print Assumptions consistency. (* confluence not proven *)
+
+(***********************************************************************************************)
+(* Strong Normalization on actual syntax *)
+
+Require TypeJudge.
+
+Module Ty := TypeJudge.
+Module Tm := Term.
+
+Fixpoint int_trm t :=
+  match t with
+  | Tm.Srt Tm.prop => SN.prop
+  | Tm.Srt Tm.kind => SN.kind
+  | Tm.Ref n => SN.Ref n
+  | Tm.App u v => SN.App (int_trm u) (int_trm v)
+  | Tm.Abs T M => SN.Abs (int_trm T) (int_trm M)
+  | Tm.Prod T U => SN.Prod (int_trm T) (int_trm U)
+  end.
+Definition interp t := int_trm (Ty.unmark_app t).
+Definition int_env := List.map interp.
+
+Section LiftAndSubstEquiv.
+(* Proof that lift and subst at both levels (SN and Tm) are equivalent. *)
+
+(* Locally Import this module *)
+Import SN.
+
+Lemma int_lift_rec : forall n t k,
+  eq_trm (lift_rec n k (int_trm t)) (int_trm (Tm.lift_rec n t k)).
+induction t; simpl int_trm; intros.
+ destruct s; simpl; trivial.
+ split; red; intros; reflexivity.
+
+ simpl; unfold V.lams, I.lams, V.shift, I.shift.
+ destruct (le_gt_dec k n0); simpl.
+  replace (k+(n+(n0-k))) with (n+n0) by omega.
+  split; red; auto.
+
+  split; red; auto.
+
+ rewrite red_lift_abs; rewrite IHt1; rewrite IHt2; reflexivity.
+ rewrite red_lift_app; rewrite IHt1; rewrite IHt2; reflexivity.
+ rewrite red_lift_prod; rewrite IHt1; rewrite IHt2; reflexivity.
+Qed.
+
+Lemma int_lift : forall n t,
+  eq_trm (int_trm (Tm.lift n t)) (lift n (int_trm t)).
+intros.
+symmetry.
+unfold Tm.lift, lift.
+apply int_lift_rec.
+Qed.
+
+
+Lemma int_subst_rec : forall arg,
+  int_trm arg <> kind ->
+  forall t k,
+  eq_trm (subst_rec (int_trm arg) k (int_trm t)) (int_trm (Tm.subst_rec arg t k)).
+intros arg not_knd.
+induction t; simpl int_trm; intros.
+ destruct s; simpl; trivial.
+ split; red; intros; reflexivity.
+
+ simpl Tm.subst_rec.
+ destruct (lt_eq_lt_dec k n) as [[fv|eqv]|bv]; simpl int_trm.
+  simpl int_trm.
+  destruct n; [inversion fv|].
+  rewrite SN.red_sigma_var_gt; auto with arith.
+  reflexivity.
+
+  subst k; rewrite SN.red_sigma_var_eq; trivial.
+  symmetry; apply int_lift.
+
+  rewrite SN.red_sigma_var_lt; trivial.
+  reflexivity.
+
+ rewrite SN.red_sigma_abs.
+ rewrite IHt1; rewrite IHt2; reflexivity.
+
+ rewrite SN.red_sigma_app.
+ rewrite IHt1; rewrite IHt2; reflexivity.
+
+ rewrite SN.red_sigma_prod.
+ rewrite IHt1; rewrite IHt2; reflexivity.
+Qed.
+
+
+Lemma int_subst : forall u t,
+  int_trm u <> kind ->
+  eq_trm (int_trm (Tm.subst u t)) (subst (int_trm u) (int_trm t)).
+unfold Tm.subst; symmetry; apply int_subst_rec; trivial.
+Qed.
+
+Lemma int_not_kind : forall T, T <> Tm.Srt Tm.kind -> interp T <> kind.
+red; intros.
+apply H.
+destruct T; try discriminate.
+destruct s; trivial; discriminate.
+destruct T1; discriminate.
+Qed.
+
+End LiftAndSubstEquiv.
+
+Hint Resolve int_not_kind Ty.eq_typ_not_kind.
+
+(* Proof that beta-reduction at the Lc level simulates beta-reduction
+   at the Tm level. One beta at the Tm level may require several
+   (but not zero) steps at the Lc level, because of the encoding
+   of type-carrying lambda abstractions.
+ *)
+Lemma red1_sound : forall x y,
+  Tm.red1 x y -> ~ Tm.mem_sort Tm.kind x ->
+  SN.red_term (int_trm x) (int_trm y).
+induction 1; simpl; intros.
+ rewrite int_subst.
+  apply SN.red_term_beta.
+
+  destruct N; try discriminate.
+  destruct s; try discriminate.
+  elim H; auto.
+
+ apply SN.red_term_abs_l; auto 10.
+ apply SN.red_term_abs_r; auto 10.
+ apply SN.red_term_app_l; auto 10.
+ apply SN.red_term_app_r; auto 10.
+ apply SN.red_term_prod_l; auto 10.
+ apply SN.red_term_prod_r; auto 10.
+Qed.
+
+Lemma sn_sound : forall M,
+  Acc (transp _ red_term) (interp M) ->
+  ~ Tm.mem_sort Tm.kind (Ty.unmark_app M) ->
+  Tm.sn (Ty.unmark_app M).
+intros M accM.
+apply Acc_inverse_image with (f:=int_trm) in accM.
+induction accM; intros.
+constructor; intros.
+apply H0; trivial.
+ apply red1_sound; trivial.
+
+ intro; apply H1; apply Tm.exp_sort_mem with (1:=H2); trivial.
+Qed.
+
+(* Soundness of the typing rules *)
+
+Lemma int_sound : forall e M M' T,
+  Ty.eq_typ e M M' T ->
+  SN.typ (int_env e) (interp M) (interp T) /\
+  SN.eq_typ (int_env e) (interp M) (interp M').
+induction 1; simpl; intros.
+ (* Srt *)
+ split.
+  apply SN.typ_prop.
+  apply SN.refl.
+ (* Ref *)
+ split.
+  destruct H0.
+  subst t.
+  unfold Tm.lift, interp; rewrite Ty.unmark_lift.
+  fold (Tm.lift (S v) (Ty.unmark_app x)); rewrite int_lift.
+  simpl.
+  apply SN.typ_var.
+  elim H1; simpl; auto.
+
+  apply SN.refl.
+ (* Abs *)
+ destruct IHeq_typ1.
+ clear IHeq_typ2.
+ destruct IHeq_typ3.
+ unfold interp; simpl; fold (interp T) (interp M) (interp U).
+ split.
+  apply SN.typ_abs; eauto.
+  destruct s1; red; auto.
+
+  apply SN.eq_typ_abs; eauto.
+ (* App *)
+ destruct IHeq_typ1.
+ destruct IHeq_typ3.
+ clear IHeq_typ2 IHeq_typ4.
+ unfold interp; simpl; fold (interp u) (interp v) (interp Ur).
+ split.
+  rewrite Ty.unmark_subst0 with (1:=H2).
+  rewrite int_subst; fold (interp v); eauto.
+  fold (interp Ur).
+  apply SN.typ_app with (interp V); eauto.
+
+  apply SN.eq_typ_app; trivial.
+ (* Prod *)
+ destruct IHeq_typ1.
+ destruct IHeq_typ2.
+ unfold interp; simpl; fold (interp T) (interp U) (interp T') (interp U').
+ split.
+  apply SN.typ_prod; trivial.
+   destruct s2; auto.
+
+   destruct s1; red; auto.
+
+  apply SN.eq_typ_prod; eauto.
+ (* Beta *)
+ destruct IHeq_typ1.
+ destruct IHeq_typ2.
+ destruct IHeq_typ3.
+ clear IHeq_typ4.
+ unfold interp; simpl; fold (interp T) (interp M) (interp U) (interp N).
+ split.
+  rewrite Ty.unmark_subst0 with (1:=H2).
+  rewrite int_subst; fold (interp N); eauto.
+  fold (interp U).
+  apply SN.typ_beta; eauto.
+  destruct s1; red; auto.
+
+  rewrite Ty.unmark_subst0 with (1:=Ty.typ_refl2 _ _ _ _ H1).
+  rewrite int_subst; fold (interp N').
+  2:assert (h := Ty.typ_refl2 _ _ _ _ H); eauto.
+  apply SN.eq_typ_beta; eauto.
+ (* Red *)
+ destruct IHeq_typ1.
+ destruct IHeq_typ2.
+ split; trivial.
+ apply SN.typ_conv with (interp T); eauto.
+ apply Ty.typ_refl2 in H0; eauto.
+ (* Exp *)
+ destruct IHeq_typ1.
+ destruct IHeq_typ2.
+ split; trivial.
+ apply SN.typ_conv with (int_trm (Ty.unmark_app T')); eauto.
+  apply SN.sym; trivial.
+
+  fold (interp T').
+  apply Ty.typ_refl2 in H0; eauto.
+Qed.
+
+  Lemma interp_wf : forall e, Ty.wf e -> SN.wf (int_env e).
+induction e; simpl; intros.
+ apply SN.wf_nil.
+
+ inversion_clear H.
+ assert (wfe := Ty.typ_wf _ _ _ _ H0).
+ apply int_sound in H0.
+ destruct H0 as (H0,_).
+ apply SN.wf_cons; auto.
+ destruct s; [left|right]; assumption.
+Qed.
+
+Lemma interp_sound : forall e M M' T,
+  Ty.eq_typ e M M' T ->
+  SN.wf (int_env e) /\ SN.typ (int_env e) (interp M) (interp T).
+intros.
+assert (wfe := Ty.typ_wf _ _ _ _ H).
+apply interp_wf in wfe.
+apply int_sound in H; destruct H; auto.
+Qed.
+
+(***********)
+(* stdlib! *)
+(*
+Lemma clos_trans_transp : forall A R x y,
+  clos_trans A R x y ->
+  clos_trans A (transp _ R) y x.
+induction 1.
+ apply t_step; trivial.
+ apply t_trans with y; trivial.
+Qed.
+*)
+
+(* The main theorem: strong normalization *)
+Theorem strong_normalization : forall e M M' T,
+  Ty.eq_typ e M M' T ->
+  Tm.sn (Ty.unmark_app M).
+Proof.
+intros.
+assert (~ Tm.mem_sort Tm.kind (Ty.unmark_app M)).
+ apply Ty.eq_typ_typ in H.
+ red; intro Hm; apply (Types.typ_mem_kind _ _ _ Hm H).
+apply interp_sound in H; destruct H as (wfe,ty).
+apply SN.model_strong_normalization in ty; trivial.
+apply sn_sound; trivial.
+Qed.
+
+(* Print the assumptions made to derive strong normalization of CC:
+   the axioms of ZF. (In fact we don't need full replacement, only the
+   functional version, so we should be able to have the SN theorem without
+   assumption.)
+ *)
+Print Assumptions strong_normalization.
