ZFfixrec.v
@@ -201,6 +201,65 @@ Existing Instance REC_morph.
    the ordinal (to determine the domain of the function used for recursive calls)
    but the result shouldn't depend on it. This is called "stage irrelevance". *)
 
+Section RecGen.
+  Variable ord : set.
+  Variable oord : isOrd ord.
+
+Let oordlt := fun o olt => isOrd_inv _ o oord olt.
+
+  Variable P : set -> set -> Prop. 
+  Hypothesis Pm : Proper (eq_set ==> eq_set ==> iff) P.
+(*
+  Hypothesis Pcont : forall o f,
+    isOrd o ->
+    o \incl ord ->
+    (forall o', o' \in o -> P (osucc o') f) ->
+    P o f.
+*)
+  Hypothesis Pcont' : forall o f,
+    morph1 f ->
+    isOrd o ->
+    o \incl ord ->
+    (forall o', o' \in o -> P (osucc o') (f o')) ->
+(* directed... *)
+    P o (sup o f).
+
+  Variable F : set -> set -> set.
+
+  Hypothesis Fm : morph2 F.
+
+  Hypothesis Ftyp : forall o f,
+    isOrd o -> o \incl ord ->
+    P o f ->
+    P (osucc o) (F o f).
+(*
+  Variable compat : set -> set -> set -> Prop.
+  Hypothesis compat_morph : Proper (eq_set ==> eq_set ==> eq_set ==> iff) compat.
+
+  Definition stage_irrelevance :=
+    forall o o' f g,
+    o' \incl ord ->
+    o \incl o' ->
+    P o f -> P o' g ->
+    compat o f g ->
+    compat (osucc o) (F o f) (F o' g).
+
+  Hypothesis Firrel : stage_irrelevance.
+*)
+
+  Lemma REC_inv_gen : forall z, isOrd z -> z \incl ord -> P z (REC F z).
+induction 1 using isOrd_ind; intros.
+rewrite REC_eq; trivial.
+apply Pcont'; trivial.
+ do 2 red; intros.
+ apply Fm; trivial.
+ apply REC_morph; trivial.
+
+ intros.
+ apply Ftyp; auto.
+ apply isOrd_inv with y; trivial.
+Qed.
+End RecGen.
 
 Section Recursor.
 
